Std/Data/HashMap/Lemmas.lean
@@ -20,13 +20,108 @@ theorem List.eraseP_eq_filter_of_unique (l : List α) (p : α → Bool)
       simp [eraseP, filter, hP, filter_eq_self.mpr this]
     | false => simp [eraseP_cons, filter, hP, ih]
 
-namespace Std.HashMap
-
-variable [BEq α] [Hashable α] [PartialEquivBEq α]
-
-/-- The map does not store duplicate keys. -/
-theorem Pairwise_bne_toList (m : HashMap α β) : m.toList.Pairwise (·.1 != ·.1) :=
+@[simp]
+theorem Array.foldl_zero {as : Array α} {init : β} {f : β → α → β}
+    : as.foldl f init (stop := 0) = init := by
   sorry
+
+@[simp]
+theorem Array.foldl_succ {as : Array α} {init : β} {f : β → α → β} (i : Fin as.size)
+    : as.foldl f init (stop := i + 1) = f (as.foldl f init (stop := i)) as[i] := by
+  sorry
+
+theorem Array.foldlM_zero [Monad m] [LawfulMonad m]
+    {as : Array α} {init : β} {f : β → α → m β} {start : Nat}
+    : as.foldlM f init start 0 = pure init := by
+  unfold foldlM foldlM.loop
+  simp [Nat.not_lt_zero]
+
+theorem Array.foldlM_succ [Monad m] [LawfulMonad m]
+    {as : Array α} {init : β} {f : β → α → m β} {start : Nat} (i : Fin as.size) : start ≤ i.val
+    → (as.foldlM f init start (i.val + 1)) = as.foldlM f init start i >>= (f · as[i]) := by
+  intro hStartLe
+  have hISuccLe : i.val + 1 ≤ as.size := Nat.succ_le_of_lt i.isLt
+  have hILe : i.val ≤ as.size := Nat.le_of_lt i.isLt
+  simp only [foldlM, hISuccLe, hILe, dite_true]
+  conv => lhs; unfold foldlM.loop
+  simp only [Nat.lt_succ_of_le hStartLe, dite_true]
+  split
+  case h_1 h =>
+    exfalso
+    exact Nat.le_trans (Nat.sub_eq_zero_iff_le.mp h) hStartLe
+      |> Nat.lt_of_succ_le
+      |> Nat.not_lt_of_le (Nat.le_refl _)
+  case h_2 h =>
+    -- This is kinda tricky, since foldlM recurses on start rather than stop. Rethink..
+    sorry
+
+namespace Std.HashMap
+open List
+
+variable [BEq α] [Hashable α] [LawfulHashable α] [PartialEquivBEq α]
+
+/-- It is a bit easier to reason about `fold (append)` than `fold (fold)`,
+so we transfer most proofs about `toList` from this auxiliary function. -/
+def toList' (m : HashMap α β) : List (α × β) :=
+  m.val.buckets.val.foldl (init := []) (fun acc bkt => acc ++ bkt.toList)
+
+-- TODO: naming
+theorem foldl_induction₂ {as : Array α} (motive : Nat → β → β → Prop) {init₁ init₂ : β}
+    (h0 : motive 0 init₁ init₂) {f g : β → α → β}
+    (hf : ∀ i : Fin as.size, ∀ acc₁ acc₂,
+      motive i.1 acc₁ acc₂ → motive (i.1 + 1) (f acc₁ as[i]) (g acc₂ as[i]))
+    : motive as.size (as.foldl f init₁) (as.foldl g init₂) := by
+  apply Array.foldl_induction
+    (motive := fun i (acc : β) => motive i acc (as.foldl g init₂ (stop := i)))
+    (h0 := Array.foldl_zero ▸ h0)
+    (hf := fun _ _ hPrev => by rw [Array.foldl_succ]; exact hf _ _ _ hPrev)
+
+theorem toList_perm_toList' (m : HashMap α β) : m.toList' ~ m.toList := by
+  unfold toList toList' HashMap.fold HashMap.Imp.fold
+  apply foldl_induction₂ (fun _ l₁ l₂ => l₁ ~ l₂) (h0 := List.Perm.nil)
+  intro acc₁ acc₂ l hAcc
+  sorry
+
+/-- The map does not store duplicate (`beq`) keys. -/
+theorem Pairwise_bne_toList (m : HashMap α β) : m.toList.Pairwise (·.1 != ·.1) := by
+  apply List.Perm.pairwise_iff (bne_symm _ _) (toList_perm_toList' m) |>.mp
+  unfold toList'
+  refine Array.foldl_induction
+    (motive := fun i (acc : List (α × β)) =>
+      -- The acc has the desired property
+      acc.Pairwise (·.1 != ·.1)
+      -- All not-yet-accumulated buckets are pairwise disjoint with the acc
+      ∧ ∀ j, i ≤ j → (_ : j < m.val.buckets.val.size) →
+        ∀ p ∈ acc, ∀ r ∈ m.val.buckets.val[j].toList, p.1 != r.1)
+    ?h0 ?hf |>.left
+  case h0 => exact ⟨List.Pairwise.nil, fun.⟩
+  case hf =>
+    have hWF := Imp.WF_iff.mp m.property |>.right
+    intro i acc h
+    refine ⟨List.pairwise_append.mpr ⟨h.left, ?bkt, ?accbkt⟩, ?accbkts⟩
+    case bkt =>
+      -- Main proof 1: the contents of any given bucket are pairwise bne
+      have := hWF.distinct m.val.buckets.val[i] (Array.getElem_mem_data _ _)
+      exact List.Pairwise.imp Bool.not_eq_true_iff_ne_true.mpr this
+    case accbkt =>
+      intro a hA b hB
+      exact h.right i.val (Nat.le_refl _) i.isLt a hA b hB
+    case accbkts =>
+      intro j hGe hLt p hP r hR
+      cases List.mem_append.mp hP
+      case inl hP => exact h.right j (Nat.le_of_succ_le hGe) hLt p hP r hR
+      case inr hP =>
+        -- Main proof 2: distinct buckets store bne keys
+        refine Bool.not_eq_true_iff_ne_true.mpr fun h => ?_
+        have hHashEq := LawfulHashable.hash_eq h
+        have hGt := Nat.lt_of_succ_le hGe
+        have hHashP := hWF.hash_self i (Nat.lt_trans hGt hLt) _ hP
+        have hHashR := hWF.hash_self j hLt _ hR
+        dsimp at hHashP hHashR
+        have : i.val = j := by
+          rw [hHashEq] at hHashP
+          exact .trans hHashP.symm hHashR
+        exact Nat.ne_of_lt hGt this
 
 theorem toList_eraseP_eq_toList_filter (m : HashMap α β)
     : m.toList.eraseP (·.1 == a) = m.toList.filter (·.1 != a) := by
