Std/Classes/BEq.lean
@@ -3,6 +3,7 @@ Copyright (c) 2022 Mario Carneiro. All rights reserved.
 Released under Apache 2.0 license as described in the file LICENSE.
 Authors: Mario Carneiro
 -/
+import Std.Logic
 
 /-! ## Boolean equality -/
 
@@ -16,6 +17,10 @@ class PartialEquivBEq (α) [BEq α] : Prop where
   symm : (a : α) == b → b == a
   /-- Transitivity for `BEq`. If `a == b` and `b == c` then `a == c`. -/
   trans : (a : α) == b → b == c → a == c
+
+theorem bne_symm [BEq α] [PartialEquivBEq α] (a b : α) : a != b → b != a :=
+  fun h => Bool.not_eq_true_iff_ne_true.mpr fun h' =>
+    Bool.not_bne_of_beq (PartialEquivBEq.symm h') h
 
 @[simp] theorem beq_eq_false_iff_ne [BEq α] [LawfulBEq α]
     (a b : α) : (a == b) = false ↔ a ≠ b := by
